



$$\left[\begin{array}{l} 1 - x = e \cdot x, y = p \cdot y \\ w = p \cdot x + p \cdot w - e \cdot x \quad h = e \cdot y - p \cdot y \end{array} \right.$$

$$\left[\begin{array}{l} 2 - x = e \cdot x + e \cdot w, y = e \cdot y \\ w = p \cdot x + p \cdot w - e \cdot x + e \cdot w, h = p \cdot y + p \cdot h - e \cdot y \end{array} \right.$$

$$\left[\begin{array}{l} 3 - x = p \cdot x, y = e \cdot y + e \cdot h \\ w = e \cdot x + e \cdot w - p \cdot x \quad h = p \cdot y + p \cdot h - e \cdot y + e \cdot h \end{array} \right.$$

$$\left[\begin{array}{l} 4 - x = p \cdot x, y = p \cdot y \\ w = e \cdot x - p \cdot x, h = e \cdot y + e \cdot h - p \cdot y \end{array} \right.$$